fixed a bug in consensusAcceptableTxG

monadproofs/proofs/reservebal.v
@@ -116,33 +116,38 @@ Definition emptyingCheckRange (knownBlocks: gmap N Block) (tx: TxWithHdr) :=
                                                                  ++  prevTxsInSameBlock).
 
 Definition isAllowedToEmpty (knownBlocks: gmap N Block)
-  (state : StateOfAccounts) (stateBlockIndex: N)  (tx: TxWithHdr) : bool :=
+  (state : StateOfAccounts) (intermediateTxsSinceState: list TxWithHdr)  (tx: TxWithHdr) : bool :=
   let notDelegated := negb (addrDelegated state (sender tx)) &&
-    forallb (fun txx => negb (txDelegatesAddr (sender tx) txx)) (intermediateTxs knownBlocks stateBlockIndex tx) in
+                        forallb (fun txx => negb (txDelegatesAddr (sender tx) txx)) intermediateTxsSinceState in
   let prevTxsFromSameSender := 
     List.filter (fun t => bool_decide (sender t = sender tx)) (emptyingCheckRange knownBlocks tx)
                 in notDelegated && bool_decide (lengthN prevTxsFromSameSender = 0).
-  
 
-Definition consensusAcceptableTxG (knownBlocks: gmap N Block) (latestState : StateOfAccounts) (intermediate: list TxWithHdr) (candidate : TxWithHdr) : bool :=
-  let bal0 := balanceOfAc latestState (sender candidate) in
-  let NminusK := (txBlockNum candidate - K) in
-  match List.filter (fun tx: TxWithHdr  => bool_decide (sender tx = sender candidate)) intermediate with
-  | [] =>
-      let reserve := staticReserveBal `min` bal0 in
-      if addrDelegated latestState (sender candidate) then
-          bool_decide (maxTxFee candidate <= balanceOfAc latestState (sender candidate))
-      else bool_decide (maxTxFee candidate ≤ reserve)
-  | t0 :: rest =>
-      if (isAllowedToEmpty knownBlocks latestState NminusK t0) 
-      then
-       let bal1 := bal0 - value t0 - maxTxFee t0 in
-       let reserve := staticReserveBal `min` bal1 in
-       bool_decide (sum_gas_bids  (candidate::rest) ≤ reserve)
-      else
-       let reserve := staticReserveBal `min` bal0 in
-       bool_decide (sum_gas_bids (candidate::intermediate) ≤ reserve)
+
+Definition maxTotalReserveDippableDebit (knownBlocks: gmap N Block) (latestKnownState : StateOfAccounts) (intermediateTxsSinceState: list TxWithHdr) tx :=
+  maxTxFee tx +
+  (if isAllowedToEmpty knownBlocks latestKnownState intermediateTxsSinceState tx
+  then value tx 
+   else 0).
+
+Fixpoint maxTotalReserveDippableDebitL (knownBlocks: gmap N Block) (latestKnownState : StateOfAccounts) (postStateAccountedSuffix rest: list TxWithHdr) (a: evm.address) : N:=
+  match rest with
+  | [] => 0
+  | h::tl =>
+      (maxTotalReserveDippableDebitL knownBlocks latestKnownState (postStateAccountedSuffix++[h]) tl a)
+      + (if bool_decide (sender h = a)
+         then (maxTotalReserveDippableDebit knownBlocks latestKnownState postStateAccountedSuffix h)
+         else 0)
   end.
+
+Definition consensusAcceptableTxG (knownBlocks: gmap N Block) (latestKnownState : StateOfAccounts) (intermediateTxsSinceState: list TxWithHdr) (candidate : TxWithHdr) : bool :=
+  let bal0 := balanceOfAc latestKnownState (sender candidate) in
+  let NminusK := (txBlockNum candidate - K) in
+  if isAllowedToEmpty knownBlocks latestKnownState intermediateTxsSinceState candidate
+  then bool_decide (maxTxFee candidate <= balanceOfAc latestKnownState (sender candidate))
+  else
+    bool_decide (maxTotalReserveDippableDebitL knownBlocks latestKnownState [] intermediateTxsSinceState (sender candidate)
+                 <= balanceOfAc latestKnownState (sender candidate)).
 
 Definition consensusAcceptableTx (knownBlocks: gmap N Block) (stateNminusK : StateOfAccounts) (candidate : TxWithHdr) : bool :=
   let NminusK := (txBlockNum candidate - K) in
@@ -175,7 +180,7 @@ Definition execTxAfterValidationV2 (knownBlocks: gmap N Block) (s: evm.GlobalSta
     bool_decide (erb  - (if bool_decide (sender t =a ) then maxTxFee t else 0) <= balanceOfAc si a) in
   let allBalCheck := (forallb balCheck allAccounts) in
   if (isAllowedToEmptyLatestState knownBlocks s t || allBalCheck)
-  then (applyGasRefundsAndRewards hdr si r, r)
+  then (applyGasRefundsAndRewards hdr si r, r) (* this cannot debit any account. move such steps to stateAfterTransactionAux *)
   else (updateBalanceOfAc s (sender t) (fun oldBal => oldBal - txMaxFee (fst (snd t))),  DippedTooMuchIntoReserve (fst (snd t))) (* revert tx *).
 
 
@@ -205,9 +210,33 @@ Lemma isEmptyingEq (knownBlocks: gmap N Block) (s1 s2 : StateOfAccounts) n tx :
   (forall a, addrDelegated s1 a = addrDelegated s2 a)
   -> isAllowedToEmpty knownBlocks s1 n tx =  isAllowedToEmpty knownBlocks s2 n tx.
 Proof using.
-  
-Admitted.
+  intros Hd.
+  unfold isAllowedToEmpty.
+  rewrite Hd.
+  reflexivity.
+Qed.
 
+Lemma maxTotalReserveDippableDebitLeq (knownBlocks: gmap N Block) (s1 s2 : StateOfAccounts) (accountedSuffix unaccountedSuffix: list TxWithHdr) (candidate : TxWithHdr) :
+  (∀ a : evm.address, addrDelegated s1 a = addrDelegated s2 a)
+  -> maxTotalReserveDippableDebitL knownBlocks s1 accountedSuffix unaccountedSuffix (sender candidate)
+     = maxTotalReserveDippableDebitL knownBlocks s2 accountedSuffix unaccountedSuffix (sender candidate).
+Proof using.
+  intros Hd. revert accountedSuffix.
+  induction unaccountedSuffix; simpl in *; auto;[].
+  intros.
+  rewrite IHunaccountedSuffix.
+  f_equal.
+  case_bool_decide; auto.
+Set Nested Proofs Allowed.
+Lemma maxTotalReserveDippableDebitEq (knownBlocks: gmap N Block) (s1 s2 : StateOfAccounts) (accountedSuffix: list TxWithHdr) (candidate : TxWithHdr) :
+  (∀ a : evm.address, addrDelegated s1 a = addrDelegated s2 a)
+  -> maxTotalReserveDippableDebitL knownBlocks s1 accountedSuffix accountedSuffix (sender candidate)
+   = maxTotalReserveDippableDebitL knownBlocks s2 accountedSuffix accountedSuffix (sender candidate).
+Proof using.
+  maxTotalReserveDippableDebit knownBlocks s1 accountedSuffix a =
+  maxTotalReserveDippableDebit knownBlocks s2 accountedSuffix a
+  
+  go.
 Lemma consensusAcceptableTxGmono (knownBlocks: gmap N Block) (s1 s2 : StateOfAccounts) (intermediate: list TxWithHdr) (candidate : TxWithHdr) :
   (forall a, balanceOfAc s1 a <= balanceOfAc s2 a)
   -> (forall a, addrDelegated s1 a = addrDelegated s2 a)
@@ -217,13 +246,14 @@ Proof.
   intros Hb Hd Hc.
   unfold consensusAcceptableTxG in *.
   specialize (Hb (sender candidate)).
-  case_match. (* filter nil *)
+  rewrite -> isEmptyingEq with (s2:=s1) by auto.
+  case_match; rewrite -> bool_decide_eq_true in *; try lia;[].
   {
+    
     rewrite <- Hd.
     destruct (addrDelegated s1 (sender candidate)); rewrite -> bool_decide_eq_true in *; lia.
   }
   {
-    rewrite -> isEmptyingEq with (s2:=s1) by auto.
     destruct (isAllowedToEmpty knownBlocks s1 (txBlockNum candidate - K) t);
       rewrite -> bool_decide_eq_true in *; try lia.
   }
@@ -238,6 +268,11 @@ Lemma inductiveStep (knownBlocks: gmap N Block) (latestState : StateOfAccounts) 
          consensusAcceptableTxG knownBlocks si intermediateTl candidate = true
      end.
 Proof.
+  intros Hc.
+  unfold consensusAcceptableTxG in Hc.
+  case_match.
+  {
+    
 
   here
 Abort.
